theories/Languages/Lustre.v
@@ -18,7 +18,7 @@ Inductive type : Set :=
 Lemma type_dec (x y: type): {x = y} + {x <> y}.
 Proof.
   destruct x, y; try solve [left; reflexivity]; right; discriminate.
-Qed.
+Defined.
 Definition sig2T_eq_type := @sig2T_eq _ type_dec.
 Arguments sig2T_eq_type {_ _ _ _}.
 
@@ -56,7 +56,7 @@ Proof.
   left.
   f_equal.
   all: assumption.
-Qed.
+Defined.
 Definition sig2T_eq_binder := @sig2T_eq _ binder_dec.
 Arguments sig2T_eq_binder {_ _ _ _}.
 
@@ -71,7 +71,7 @@ Lemma const_inv {ty} (x: const ty) :
   {exists (eq : ty = _), x = eq_rect _ const CVoid _ (eq_sym eq)}.
 Proof using.
   destruct x as [|b|n]; [right|left; left|left; right]; exists eq_refl; [|exists b|exists n]; exact eq_refl.
-Qed.
+Defined.
 Lemma const_dec {ty} (x y: const ty) : {x = y} + {x <> y}.
 Proof.
   destruct x as [ | b | n ].
@@ -82,7 +82,7 @@ Proof.
   4: destruct (PeanoNat.Nat.eq_dec n n') as [eq|ne]; [left|right].
   all: rewrite !(Eqdep_dec.UIP_dec type_dec _ eq_refl); cbn; try intros [=f]; auto.
   exact (f_equal _ eq).
-Qed.
+Defined.
 
 (** A unary operator
 
@@ -99,7 +99,7 @@ Lemma unop_inv {ty tout} (x: unop ty tout) :
   {exists (eq1 : ty = TInt) (eq2 : tout = TInt), x = eq_rect _ (unop _) (eq_rect _ (fun ty => unop ty _) Uop_neg _ (eq_sym eq1)) _ (eq_sym eq2)}.
 Proof using.
   destruct x; [left|right]; exists eq_refl, eq_refl; exact eq_refl.
-Qed.
+Defined.
 Lemma unop_dec {ty tout} (x y: unop ty tout) : {x = y} + {x <> y}.
 Proof.
   destruct (unop_inv x) as [H1|H1].
@@ -112,7 +112,7 @@ Proof.
   all: rewrite !(Eqdep_dec.UIP_dec type_dec _ eq_refl); cbn.
   1-2: reflexivity.
   all: discriminate.
-Qed.
+Defined.
 
 (** A binary operator
 
@@ -167,7 +167,7 @@ Proof using.
   1-01: left.
   2-12: right.
   all: exists eq_refl, eq_refl, eq_refl; exact eq_refl.
-Qed.
+Defined.
 Lemma binop_dec {ty1 ty2 tout} (x y: binop ty1 ty2 tout) : {x = y} + {x <> y}.
 Proof.
   pose proof (binop_inv x) as H1.
@@ -245,7 +245,7 @@ Proof.
   all: try solve [repeat (rewrite (Eqdep_dec.UIP_dec type_dec _ eq_refl) in f; cbn in f); discriminate f].
   all: destruct f as [? [? [? f]]]; try discriminate.
   all: repeat (rewrite (Eqdep_dec.UIP_dec type_dec _ eq_refl) in f; cbn in f); discriminate f.
-Qed.
+Defined.
 
 Inductive exp : type -> Set :=
   | EConst: forall {ty}, const ty -> exp ty
@@ -273,7 +273,7 @@ Proof using.
   2-6: right.
   all: try solve [repeat eexists; exact eq_refl].
   1,2: exists b, eq_refl; exact eq_refl.
-Qed.
+Defined.
 Lemma exp_dec {ty} (e1 e2: exp ty) : {e1 = e2} + {e1 <> e2}.
 Proof.
   revert e2.
@@ -317,7 +317,7 @@ Proof.
     destruct (IHt et2) as [<-|ne]; [|right; intros [=f]; exact (ne (sig2T_eq_type f))].
     destruct (IHf ef2) as [<-|ne]; [|right; intros [=f]; exact (ne (sig2T_eq_type f))].
     left; reflexivity.
-Qed.
+Defined.
 
 Fixpoint has_einput {ty} (e: exp ty): bool :=
   match e with
@@ -339,7 +339,7 @@ Proof.
   destruct (type_dec ty1 ty2) as [<-|ne]; [|right; cbn; intros [=f]; exact (ne f)].
   destruct (exp_dec e1 e2) as [<-|ne]; [|right; cbn; intros [=f]; exact (ne (sig2T_eq_type f))].
   left; reflexivity.
-Qed.
+Defined.
 
 Record node := mk_node {
   n_name: string;
@@ -392,7 +392,7 @@ Proof using.
   2-5: right.
   all: try solve [repeat eexists; exact eq_refl].
   exists b, eq_refl; exact eq_refl.
-Qed.
+Defined.
 Lemma value_dec {ty} (e1 e2: value ty) : {e1 = e2} + {e1 <> e2}.
 Proof.
   revert e2.
@@ -429,7 +429,7 @@ Proof.
     destruct (IHt et2) as [<-|ne]; [|right; intros [=f]; exact (ne (sig2T_eq_type f))].
     destruct (IHf ef2) as [<-|ne]; [|right; intros [=f]; exact (ne (sig2T_eq_type f))].
     left; reflexivity.
-Qed.
+Defined.
 
 Definition history := Dict.t {ty & Stream.t (value ty)}.
 Definition in_history (h : history) '((v, ty) : nat * type) := match Dict.find v h with
